\begin{answer}
For simplicity we write  $\nabla_{\theta}l(\theta) =\nabla_{\theta'}l(\theta)|_{\theta' = \theta}. $
Using Taylor we have
$$
l(\theta+ d) \approx l(\theta) + d^T\nabla_{\theta}l(\theta)
$$
We can construct the Lagrangian for this optimization problem as
$$
\begin{aligned}
\mathcal L(d, \lambda) &= l(\theta+d)  - \lambda[D_{KL}(p_{\theta}\|p_{\theta + d}) - c]\\
&= l(\theta) + d^T\nabla_{\theta}l(\theta) - \lambda[\frac{1}{2}d^T\mathcal I(\theta)d - c]
\end{aligned}
$$
By using the Lagrange multiplier method we have
$$
\begin{aligned}
\frac{\partial \cal L}{\partial d} &=  \nabla_{\theta}l(\theta) - \lambda \mathcal I(\theta)d = 0\\
\frac{\partial \cal L}{\partial \lambda} &= \frac{1}{2}d^T\mathcal I(\theta) d - c = 0
\end{aligned}
$$
We find $d$ from the first equation
$$
d = \frac{1}{\lambda}\mathcal I(\theta)^{-1}\nabla_{\theta'}l(\theta)
$$
We plug in the above $d$ into the second equation.


$$
\frac{1}{2}(\frac{1}{\lambda^2}(\mathcal I(\theta)^{-1})^T\nabla^T_{\theta}l(\theta)\mathcal I(\theta)\mathcal I(\theta)^{-1}\nabla_{\theta}l(\theta) = c
$$
Solve for $\lambda$
$$
\lambda = \sqrt{\frac{1}{2c}(\nabla^T_{\theta}l(\theta)\mathcal I(\theta)^{-1} \nabla_{\theta}l(\theta))}
$$
Now, we find $d^{*}$
$$
d^{*} =\sqrt{\frac{2c}{\nabla^T_{\theta}l(\theta)\mathcal I(\theta)^{-1} \nabla_{\theta}l(theta)}}\mathcal I(\theta)^{-1}\nabla_{\theta}l(\theta).
$$


 \end{answer}
