\begin{answer}
Apply Bayes
$$p(y = 1| x) = \frac{p(x| y=1)p(y = 1)}{p(x| y=1)p(y = 1) + p(x| y=0)p(y = 0)} = \frac{1}{1 + \frac{p(x| y=0)p(y = 0)}{p(x| y=1)p(y = 1)}}.$$
Note that $\frac{p(y = 0)}{p(y = 1)} = exp(ln(\frac{1-\phi}{\phi})$
For simplicity  denote A = $\Sigma^{-1}.$
Note that
$$\frac{p(x| y=0)}{p(x| y=1)} = exp(-\frac{1}{2}(A(x- \mu_0), x - \mu_0) - (A(x- \mu_1), x - \mu_1))) $$$$= exp(-\frac 12((Ax,x) - 2(Ax, \mu_0) + (\mu_0, \mu_0) - (Ax,x) + 2(Ax, \mu_1) + (\mu_1, \mu_1)))$$
$$= exp(-( -(Ax, \mu_0) + \frac 12(A\mu_0, \mu_0) + (Ax, \mu_1) - \frac12(A\mu_1, \mu_1))) = exp(-(\mu_1 - \mu_0)^TAx + \frac{1}{2}((A\mu_0,\mu_0) - (A\mu_1,\mu_1)).$$
From this we find $\theta^T = (\mu_1 - \mu_0)^TA$ hence 
$$\theta = (\Sigma^{-1})^T(\mu_1 - \mu_0)$$
and
$$\theta_0 = \frac{1}{2}((\Sigma^{-1}\mu_0,\mu_0) - (\Sigma^{-1}\mu_1,\mu_1)) - ln(\frac{1-\phi}{\phi}).$$

\end{answer}
