\begin{answer}
We apply the following inequality
$$\log x \le x - 1 \text(for)  0< x\le 1.$$
In addition, the equality holds if and only is $x = 1.$ To prove this,
note that the function $f(x) = \log x - x + 1$ for $0< x \le 1$ is increasing and $f(1) = 0.$
This means that $f(x) <= 0$ for $0< x\le .$
Now
$$D_{KL}(P,Q) = - \sum\limits_x P(x)\log\frac{Q(x)}{P(x)} \ge \sum\limits_x P(x)(\frac{Q(x)}{P(x)} - 1)=$$
$$ = \sum\limits_x (Q(x) - P(x)) = 1- 1 = 0.$$
In addition, the equality holds if and only if $\frac{Q(x)}{P(x)} = 1,$ hence $P(x) = Q(x)$
\end{answer}
